finish adequacy for schedule conditions

theories/program_logic/adequacy.v
@@ -1,118 +1,313 @@
 From iris.proofmode Require Import tactics.
-From iris.base_logic.lib Require Import wsat.
+From iris.base_logic.lib Require Import wsat invariants saved_prop.
+From iris.algebra Require Import auth excl gmap.
 From machine_program_logic.program_logic Require Export weakestpre.
 Import uPred.
+
+(* move to stdpp *)
+Section big_opL.
+  Context {M : ofe} (o : M → M → M) `{!Monoid o}.
+
+  Lemma big_opL_filter {A} (φ : A → M) (P : A → Prop) `{!∀ a, Decision (P a)} l :
+    ([^o list] a ∈ filter P l, φ a) ≡
+    [^o list] a ∈ l, if bool_decide (P a) then φ a else monoid_unit.
+  Proof.
+    induction l as [|a l IHl]; simpl; first done.
+    destruct (decide (P a)).
+    - rewrite filter_cons_True; last done.
+      rewrite bool_decide_eq_true_2; last done.
+      rewrite /=.
+      apply ne_proper_2; [apply monoid_ne|done|done].
+    - rewrite filter_cons_False; last done.
+      rewrite bool_decide_eq_false_2; last done.
+      rewrite monoid_left_id; done.
+  Qed.
+
+  Lemma big_opL_seq {A} s n (φ : nat → M) (l : list A) :
+    n = length l →
+    ([^o list] a ∈ seq s n, φ a) ≡ [^o list] i ↦ _ ∈ l, φ (s + i).
+  Proof.
+    revert s l; induction n as [|n IHn]; intros s l Hnl; first by destruct l.
+    destruct l; simpl in *; first done.
+    rewrite Nat.add_0_r.
+    apply ne_proper_2; [apply monoid_ne|done|].
+    setoid_rewrite <- Nat.add_succ_comm; eauto.
+  Qed.
+
+End big_opL.
+
+(* also move to stdpp *)
+Lemma bool_decide_of_eq_true b : bool_decide (b = true) = b.
+Proof. destruct b; done. Qed.
 
 Section adequacy.
 Context `{!irisG M Σ}.
 Implicit Types m : mode M.
+Implicit Types σ : state M.
 Implicit Types P Q : iProp Σ.
 Implicit Types Φ : mode M → iProp Σ.
 Implicit Types Φs : list (mode M → iProp Σ).
 
-Notation wptp t Φs := ([∗ list] id ↦ e;Φ ∈ t;Φs, WP e @ id ; ⊤ {{ Φ }})%I.
+Definition wpvm σ id m Φ : iProp Σ :=
+  ((∃ P, VMPropAuth id P) ∗
+   if terminated m then Φ m else
+     ((if scheduled σ id then True else VMProp_holds id) -∗ WP m @ id; ⊤ {{ Φ }}))%I.
 
-Lemma wp_step id m1 σ1 m2 σ2 Φ :
+Notation wpvms_convid f σ t Φs := ([∗ list] id ↦ m;Φ ∈ t;Φs, wpvm σ (f id) m Φ)%I.
+
+Notation wpvms σ t Φs := ([∗ list] id ↦ m;Φ ∈ t;Φs, wpvm σ id m Φ)%I.
+
+Lemma wp_step n id m1 σ1 m2 σ2 Φ :
   scheduled σ1 id →
   prim_step m1 σ1 m2 σ2 →
-  state_interp σ1 -∗ WP m1 @ id; ⊤ {{ Φ }}
+  state_interp n σ1 -∗ wpvm σ1 id m1 Φ
     ={⊤,∅}=∗ |={∅}▷=> |={∅,⊤}=>
-    state_interp σ2 ∗ WP m2 @ id; ⊤ {{ Φ }}.
+    ([∗ list] vmid ∈ just_scheduled_vms n σ1 σ2, VMProp_holds vmid) ∗
+    state_interp n σ2 ∗ wpvm σ2 id m2 Φ.
 Proof.
-  rewrite {1}wp_unfold /wp_pre. iIntros (? ?) "Hσ H".
+  iIntros (? ?) "Hσ [HPA H]".
   rewrite (terminated_stuck m1 σ1 m2 σ2) //.
-  iMod ("H" $! σ1 with "[//] Hσ") as "(_ & H)". iModIntro.
-  iMod ("H" with "[//]") as "H".
+  rewrite /wpvm {1}wp_unfold /wp_pre.
+  rewrite (terminated_stuck m1 σ1 m2 σ2) //.
+  destruct (scheduled σ1 id) eqn:Hsch; last done.
+  iMod ("H" with "[//] [] Hσ") as "(_ & H)"; first by rewrite Hsch.
+  iModIntro.
+  iMod ("H" with "HPA [//]") as "H".
   iModIntro; iNext; iModIntro.
-  iMod "H" as "[$ $]"; done.
+  iMod "H" as "($ & $ & $ & H)".
+  destruct (scheduled σ2 id); destruct (terminated m2) eqn:Hterm;
+    simpl; [|done| |done]; rewrite wp_unfold /wp_pre Hterm; iApply "H"; done.
 Qed.
 
-Lemma wptp_step ms1 ms2 σ1 σ2 Φs :
-  step (ms1,σ1) (ms2, σ2) →
-  state_interp σ1 -∗
-  wptp ms1 Φs -∗
-  |={⊤,∅}=> |={∅}▷=> |={∅,⊤}=> state_interp σ2 ∗ wptp ms2 Φs.
+Lemma wpvm_step_by_other id m σ1 σ2 Φ :
+  wpvm σ1 id m Φ -∗
+  (if just_scheduled σ1 σ2 id then VMProp_holds id else emp) -∗
+  wpvm σ2 id m Φ.
 Proof.
-  iIntros (Hstep) "Hσ Ht".
-  destruct Hstep as [m1' σ1' m2' σ2' t2' t3 Hstep]; simplify_eq/=.
-  iDestruct (big_sepL2_app_inv_l with "Ht") as (Φs1 Φs2 ->) "[? Ht]".
-  iDestruct (big_sepL2_cons_inv_l with "Ht") as (Φ Φs3 ->) "[Ht ?]".
-  iMod (wp_step with "Hσ Ht") as ">H"; [by rewrite Nat.add_0_r|done|].
-  iModIntro; iModIntro; iNext; iMod "H"; iModIntro.
-  iMod "H" as "[$ ?]"; iFrame; done.
+  rewrite /wpvm.
+  iIntros "[HPA Hwp]".
+  rewrite /just_scheduled.
+  destruct (scheduled σ1 id) eqn:Hsch1; destruct (terminated m) eqn:Hsterm;
+    simpl; iFrame; [done| |by auto|].
+  - iIntros "_"; iFrame; iIntros "?"; iApply "Hwp"; done.
+  - destruct (scheduled σ2 id) eqn:Hsch2; simpl.
+    + iFrame. iIntros "? _"; iApply "Hwp"; done.
+    + iIntros "_"; iFrame.
 Qed.
 
-Lemma wptp_steps n ms1 ms2 σ1 σ2 Φs :
-  nsteps step n (ms1, σ1) (ms2, σ2) →
-  state_interp σ1 -∗ wptp ms1 Φs
-  ={⊤,∅}=∗ |={∅}▷=>^n |={∅,⊤}=> state_interp σ2 ∗ wptp ms2 Φs.
+Lemma wpvms_step_by_other f ms σ1 σ2 Φs :
+  wpvms_convid f σ1 ms Φs -∗
+  ([∗ list] id ↦ _ ∈ ms, (if just_scheduled σ1 σ2 (f id) then VMProp_holds (f id) else emp)) -∗
+  wpvms_convid f σ2 ms Φs.
+Proof.
+  iInduction ms as [|vm ms] "IH" forall (f Φs).
+  - iIntros "H". iDestruct (big_sepL2_nil_inv_l with "H") as %->; simpl; auto.
+  - iIntros "H".
+    iDestruct (big_sepL2_cons_inv_l with "H") as (Φ Φs' ->) "[Hvm Hvms]".
+    iIntros "[Hvmjsch Hvmsjsch]".
+    iSplitL "Hvm Hvmjsch"; first by iApply (wpvm_step_by_other with "[$] [$]").
+    iApply ("IH" with "[$] [$]").
+Qed.
+
+Lemma wpvms_step n ms1 ms2 σ1 σ2 Φs :
+  n = length ms1 →
+  step (ms1,σ1) (ms2, σ2) →
+  state_interp n σ1 -∗
+  wpvms σ1 ms1 Φs -∗
+  |={⊤,∅}=> |={∅}▷=> |={∅,⊤}=> state_interp n σ2 ∗ wpvms σ2 ms2 Φs.
+Proof.
+  iIntros (Hn Hstep) "Hσ Ht".
+  destruct Hstep as [m1' σ1' m2' σ2' t2' t3 Hstep]; simplify_eq/=.
+  iDestruct (big_sepL2_app_inv_l with "Ht") as (Φs1 Φs2 ->) "[Ht2' Ht]".
+  iDestruct (big_sepL2_cons_inv_l with "Ht") as (Φ Φs3 ->) "[Ht Ht3]".
+  rewrite Nat.add_0_r.
+  iMod (wp_step with "Hσ Ht") as ">H"; [by rewrite Hstep|done|].
+  iModIntro; iModIntro; iNext; iMod "H"; iModIntro.
+  iMod "H" as "(Hjsch & $ & H)".
+  iModIntro.
+  rewrite /just_scheduled_vms big_opL_filter big_opL_seq /=; last done.
+  rewrite big_sepL_app.
+  iDestruct "Hjsch" as "[Hjscht2' [Hjsch Hjscht3]]".
+  iApply (big_sepL2_app with "[Ht2' Hjscht2']").
+  { iApply (wpvms_step_by_other (λ x, x) with "[$]").
+    erewrite big_opL_ext; [done|by intros ???; rewrite bool_decide_of_eq_true]. }
+  iSplitL "H"; first by rewrite Nat.add_0_r.
+  iApply (wpvms_step_by_other with "[$]").
+  erewrite big_opL_ext; [done|by intros ???; rewrite bool_decide_of_eq_true].
+Qed.
+
+(* if we want to support dynamic creation VM's at some point we need to *)
+(* strengthen the next tow lemmas. *)
+Lemma step_preserve_vms_length ms1 σ1 ms2 σ2 :
+  step (ms1, σ1) (ms2, σ2) → length ms1 = length ms2.
+Proof.
+  inversion 1; simplify_eq.
+  rewrite !app_length; done.
+Qed.
+
+Lemma nsteps_preserve_vms_length n ms1 σ1 ms2 σ2 :
+  nsteps step n (ms1, σ1) (ms2, σ2) → length ms1 = length ms2.
+Proof.
+  revert ms1 σ1 ms2 σ2; induction n as [|n IHn]; intros ms1 σ1 ms2 σ2;
+    inversion 1 as [|?? [] ?]; subst; first done.
+  etrans; first by eapply step_preserve_vms_length.
+  eapply IHn; eauto.
+Qed.
+
+Lemma wpvms_steps k n ms1 ms2 σ1 σ2 Φs :
+  n = length ms1 →
+  nsteps step k (ms1, σ1) (ms2, σ2) →
+  state_interp n σ1 -∗ wpvms σ1 ms1 Φs
+  ={⊤,∅}=∗ |={∅}▷=>^k |={∅,⊤}=> state_interp n σ2 ∗ wpvms σ2 ms2 Φs.
 Proof.
   revert ms1 ms2 σ1 σ2 Φs.
-  induction n as [|n IH]=> em1 ms2 σ1 σ2 Φs /=.
+  induction k as [|k IHk]=> ms1 ms2 σ1 σ2 Φs Hlen /=.
   { inversion_clear 1; iIntros "? ?". iFrame.
     iMod (fupd_mask_subseteq ∅) as "H"; first done. by iFrame. }
   iIntros (Hsteps) "Hσ He". inversion_clear Hsteps as [|?? [t1' σ1']].
-  iDestruct (wptp_step with "Hσ He") as ">H"; first eauto; simplify_eq.
+  iDestruct (wpvms_step with "Hσ He") as ">H"; [done|done|].
   iModIntro. iApply step_fupd_fupd. iApply (step_fupd_wand with "H").
-  iIntros ">[Hσ He]". iMod (IH with "Hσ He") as "IH"; first done. iModIntro.
+  iIntros ">[Hσ He]".
+  iMod (IHk with "Hσ He") as "IH";
+    [by erewrite <- step_preserve_vms_length; eauto|done|iModIntro].
   iApply (step_fupdN_wand with "IH"). iIntros ">[$ $]"; done.
 Qed.
 
-Lemma wp_not_stuck id m σ Φ :
+Lemma wp_not_stuck n id m σ Φ :
   scheduled σ id →
-  state_interp σ -∗ WP m @ id {{ Φ }} ={⊤}=∗ ⌜not_stuck m σ⌝.
+  state_interp n σ -∗ WP m @ id {{ Φ }} ={⊤}=∗ ⌜not_stuck m σ⌝.
 Proof.
   rewrite wp_unfold /wp_pre /not_stuck. iIntros (?) "Hσ H".
   destruct (terminated m) eqn:?; first by eauto.
-  iSpecialize ("H" $! σ with "[//] Hσ"). rewrite sep_elim_l.
+  iSpecialize ("H" $! _ σ with "[//] Hσ"). rewrite sep_elim_l.
   iMod (fupd_plain_mask with "H") as %?; eauto.
 Qed.
 
-Lemma wptp_strong_adequacy n Φs ms1 ms2 σ1 σ2:
-  nsteps step n (ms1, σ1) (ms2, σ2) →
-  state_interp σ1 -∗ wptp ms1 Φs
-  ={⊤,∅}=∗ |={∅}▷=>^n |={∅,⊤}=>
-    ⌜ ∀ i m2, scheduled σ2 i → ms2 !! i = Some m2 → not_stuck m2 σ2 ⌝ ∗
-    state_interp σ2 ∗
+Lemma wpvms_strong_adequacy k n Φs ms1 ms2 σ1 σ2 :
+  n = length ms1 →
+  nsteps step k (ms1, σ1) (ms2, σ2) →
+  state_interp n σ1 -∗ wpvms σ1 ms1 Φs
+  ={⊤,∅}=∗ |={∅}▷=>^k |={∅,⊤}=>
+    ⌜∀ i m2, scheduled σ2 i → ms2 !! i = Some m2 → not_stuck m2 σ2⌝ ∗
+    state_interp n σ2 ∗
     [∗ list] m;Φ ∈ ms2;Φs,
       from_option Φ True (if terminated m then Some m else None).
 Proof.
-  iIntros (Hstep) "Hσ He". iMod (wptp_steps with "Hσ He") as "Hwp"; first done.
+  iIntros (Hlen Hstep) "Hσ He". iMod (wpvms_steps with "Hσ He") as "Hwp"; [done|done|].
   iModIntro. iApply (step_fupdN_wand with "Hwp").
   iMod 1 as "(Hσ & Ht)"; simplify_eq/=.
   iMod (fupd_plain_keep_l ⊤
     ⌜ ∀ i m2, scheduled σ2 i → ms2 !! i = Some m2 → not_stuck m2 σ2 ⌝%I
-    (state_interp σ2 ∗ wptp ms2 Φs)%I
+    (state_interp (length ms1) σ2 ∗ wpvms σ2 ms2 Φs)%I
     with "[$Hσ $Ht]") as "(%&Hσ&Hwp)".
   { iIntros "(Hσ & Ht)" (i m' Hm'sch Hm').
     move: Hm' => /(elem_of_list_split_length _ _ _)[?[?[-> ?]]]; subst.
     iDestruct (big_sepL2_app_inv_l with "Ht") as (Φs1 Φs2 ?) "[? Hwp]".
     iDestruct (big_sepL2_cons_inv_l with "Hwp") as (Φ Φs3 ->) "[Hwp ?]".
     rewrite Nat.add_0_r.
-    iMod (wp_not_stuck with "Hσ Hwp") as "$"; auto. }
+    iMod (wp_not_stuck with "Hσ [Hwp]") as "$"; [done| |done].
+    rewrite /wpvm.
+    iDestruct "Hwp" as "[_ Hwp]".
+    destruct terminated eqn:Hterm.
+    - rewrite wp_unfold /wp_pre Hterm; eauto.
+    - destruct scheduled; last done.
+      iApply "Hwp"; done. }
   iSplitR; first done. iFrame "Hσ".
   iApply big_sepL2_fupd.
   iApply (big_sepL2_impl with "Hwp").
-  iIntros "!#" (? m Φ ??) "Hwp".
+  iIntros "!#" (vmid m Φ ? ?) "Hwp".
   destruct (terminated m) eqn:Hm2'; last done.
-  simpl. iApply wp_terminated_inv'; done.
+  simpl. iApply (wp_terminated_inv' vmid); first done.
+  rewrite /wpvm.
+  iDestruct "Hwp" as "[_ Hwp]".
+  rewrite Hm2'.
+  rewrite wp_unfold /wp_pre Hm2'; eauto.
 Qed.
 End adequacy.
 
+Class irisPreGS (Σ : gFunctors) := IrisPreG {
+  iris_invPreGS :> invGpreS Σ;
+  irisG_saved_prop :> savedPropG Σ;
+  irisG_prop_name :> inG Σ (authUR (optionUR (exclR gnameO)));
+  irisG_name_map :> inG Σ (authUR (gmapUR nat (agreeR gnameO)));
+}.
+
+Definition irisΣ :=
+  #[invΣ; savedPropΣ; GFunctor (authUR (optionUR (exclR gnameO)));
+    GFunctor (authUR (gmapUR nat (agreeR gnameO)))].
+
+Global Instance iris_subG Σ : subG irisΣ Σ → irisPreGS Σ.
+Proof. solve_inG. Qed.
+
+Lemma allocated_props `{!irisPreGS Σ} n (N : gmap nat gname) (Ps : list (iProp Σ)) γ :
+  let VMProp γNN id P :=
+      (∃ (γvmn : gname) (γ : gnameO),
+        own γNN (◯ {[id := to_agree γvmn]})
+            ∗ own γvmn (◯ Excl' γ) ∗ saved_prop_own γ P)%I
+  in
+  let VMPropAuth γNN id P :=
+      (∃ (γvmn : gname) (γ : gnameO),
+        own γNN (◯ {[id := to_agree γvmn]})
+            ∗ own γvmn (● Excl' γ) ∗ saved_prop_own γ P)%I
+  in
+  own γ (● (to_agree <$> N : gmapUR nat (agreeR gnameO))) -∗
+  ⌜∀ k, k ∈ dom (gset nat) N ↔ k < n⌝ ==∗
+    ∃ (M : gmap nat gname),
+      ⌜∀ k, k ∈ dom (gset nat) M ↔ k < n + length Ps ⌝ ∗
+      own γ (● (to_agree <$> M : gmapUR nat (agreeR gnameO))) ∗
+      ([∗ list] id↦P ∈ Ps, VMProp γ (n + id) P) ∗
+      ([∗ list] id↦P ∈ Ps, VMPropAuth γ (n + id) P).
+Proof.
+  iIntros "Hγ %HN".
+  iInduction Ps as [|P Ps] "IH" forall (n N HN).
+  - simpl; iModIntro; iExists N; iFrame.
+    iSplit; last done.
+    iPureIntro.
+    intros ?; rewrite HN; lia.
+  - iMod (saved_prop_alloc P) as (γP) "#HP".
+    iMod (own_alloc ((● Excl' γP) ⋅ (◯ Excl' γP))) as (γPe) "[HγPeF HγPe]".
+    { apply auth_both_valid; done. }
+    iMod (own_update
+            _ _ (● (to_agree <$> <[n := γPe]>N : gmapUR nat (agreeR gnameO))
+                   ⋅ ◯ {[ n := to_agree γPe]}) with "Hγ") as "[Hγ #HγP]".
+    { rewrite fmap_insert.
+      apply auth_update_alloc, alloc_local_update; last done.
+      apply not_elem_of_dom.
+      rewrite dom_fmap HN; lia. }
+    iMod ("IH" $! (S n) _ with "[] Hγ") as (M) "(%Hdom & Hγ & HPs & HPsF)".
+    { iPureIntro; intros ?. rewrite dom_insert_L elem_of_union elem_of_singleton HN; lia. }
+    iModIntro; iExists _; iFrame "Hγ".
+    iSplit.
+    { iPureIntro; simpl; split; rewrite Hdom; lia. }
+    rewrite /= !Nat.add_0_r.
+    setoid_rewrite <- Nat.add_succ_comm.
+    iSplitR "HγPeF HPsF"; [iFrame "HPs"|iFrame "HPsF"];
+      iExists _, _; iFrame; iFrame "#".
+Qed.
+
 (** Iris's generic adequacy result *)
-Theorem wp_strong_adequacy Σ M `{!invGpreS Σ} ms1 σ1 n ms2 σ2 φ :
+Theorem wp_strong_adequacy Σ M `{!irisPreGS Σ} ms1 σ1 n ms2 σ2 φ :
   (∀ `{Hinv : !invGS Σ},
-    ⊢ |={⊤}=> ∃
-         (stateI : state M → iProp Σ)
+      ⊢ |={⊤}=>
+         ∀ name_map_name,
+         ∃
+         (stateI : nat → state M → iProp Σ)
          (Φs : list (mode M → iProp Σ)),
-       let _ : irisG M Σ := IrisG _ _ Hinv stateI in
-       stateI σ1 ∗
-       ([∗ list] id ↦ e;Φ ∈ ms1;Φs, WP e @ id; ⊤ {{ Φ }}) ∗
+         let _ : irisG M Σ := IrisG _ _ Hinv _ _ _ name_map_name stateI in
+         |={⊤}=> ∃ (Ps : list (iProp Σ)),
+       ⌜length Ps = length ms1⌝ ∗
+       stateI (length ms1) σ1 ∗
+       (([∗ list] id ↦ P ∈ Ps, VMProp id P) -∗
+           [∗ list] id ↦ m;Φ ∈ ms1;Φs,
+             if terminated m then
+                Φ m
+              else (if (scheduled σ1 id) then True else VMProp_holds id) -∗
+              WP m @ id; ⊤ {{ Φ }}) ∗
        ( (* If this is a stuck-free triple (i.e. [s = NotStuck]), then all
          threads in [t2] are not stuck *)
          ⌜ ∀ i m2, scheduled σ2 i → ms2 !! i = Some m2 → not_stuck m2 σ2 ⌝ -∗
          (* The state interpretation holds for [σ2] *)
-         stateI σ2 -∗
+         stateI (length ms1) σ2 -∗
          (* If the initial threads are done, their post-condition [Φ] holds *)
          ([∗ list] m;Φ ∈ ms2;Φs, from_option Φ True (if terminated m then Some m else None)) -∗
          (* Under all these assumptions, and while opening all invariants, we
@@ -125,10 +320,43 @@ Theorem wp_strong_adequacy Σ M `{!invGpreS Σ} ms1 σ1 n ms2 σ2 φ :
 Proof.
   intros Hwp ?.
   apply (step_fupdN_soundness _ (S n))=> Hinv.
-  iMod Hwp as (stateI Φ) "(Hσ & Hwp & Hφ)".
+  iMod Hwp as "Hwp".
+  iMod (own_alloc (● ∅)) as (name_map_name) "HNNF".
+  { apply auth_auth_valid; done. }
+  iDestruct ("Hwp" $! name_map_name) as (stateI Φs) ">Hwp".
+  clear Hwp.
+  iDestruct "Hwp" as (Ps Hlen) "(Hσ & Hwp & Hφ)".
+  iEval (rewrite -(fmap_empty to_agree)) in "HNNF".
+  iMod (allocated_props 0 ∅ Ps with "HNNF []") as (?) "(_ & HNNF & HPs & HPsF)".
+  { iPureIntro; intros ?; rewrite dom_empty; split; [set_solver|lia]. }
+  simpl.
+  iSpecialize ("Hwp" with "HPs").
+  set (IG := IrisG _ _ Hinv _ _ _ name_map_name stateI).
+  iDestruct (big_sepL2_length with "Hwp") as %HΦs.
+  iAssert ([∗ list] id↦m;_ ∈ ms1;Φs, ∃ P, VMPropAuth id P)%I with "[HPsF]" as "HPsF".
+  { clear -Ps Hlen Φs HΦs.
+    iStopProof.
+    change (([∗ list] id↦P ∈ Ps, ∃ (γvmn : gname) (γ : gnameO),
+                         own name_map_name (◯ {[0 + id := to_agree γvmn]})
+                         ∗ own γvmn (● Excl' γ) ∗ saved_prop_own γ P)
+              -∗ [∗ list] id↦_;_ ∈ ms1;Φs, ∃ P : iProp Σ, VMPropAuth (0 + id) P).
+    generalize 0 as k.
+    revert Ps Hlen Φs HΦs.
+    induction ms1 as [|m ms1 IHms1]; iIntros (Ps Hlen Φs HΦs k) "HPsF".
+    - destruct Φs; done.
+    - destruct Φs; first done.
+      destruct Ps; first done.
+      simpl in *.
+      iDestruct "HPsF" as "[HPF HPsF]".
+      iSplitR "HPsF".
+      + iExists _; iFrame.
+      + setoid_rewrite <- Nat.add_succ_comm.
+        iApply (IHms1 Ps); [lia|lia|done]. }
+  iCombine "HPsF Hwp" as "Hwp".
+  rewrite -big_sepL2_sep.
   iDestruct (big_sepL2_length with "Hwp") as %Hlen1.
-  iMod (@wptp_strong_adequacy _ _ (IrisG _ _ Hinv stateI) _ with "Hσ Hwp")
-    as "H"; first done.
+  iMod (@wpvms_strong_adequacy _ _ IG _ with "Hσ Hwp")
+    as "H"; [done|done|].
   iAssert (|={∅}▷=>^(S n) |={∅}=> ⌜φ⌝)%I with "[-]" as "H"; last first.
   { by iApply step_fupdN_S_fupd. }
   iApply (step_fupdN_wand with "H").
@@ -189,65 +417,102 @@ Proof.
   rewrite Hm2ter in Hn1; done.
 Qed.
 
-Corollary wp_adequacy Σ M `{!invGpreS Σ} ms σ φs :
+Corollary wp_adequacy Σ M `{!irisPreGS Σ} ms σ φs :
+  length ms = length φs →
   (∀ `{Hinv : !invGS Σ},
-     ⊢ |={⊤}=> ∃
-         (stateI : state M → iProp Σ),
-       let _ : irisG M Σ :=
-           IrisG _ _ Hinv stateI
-       in
-       stateI σ ∗ ([∗ list] id ↦ e;Φ ∈ ms;φs, WP e @ id; ⊤ {{v, ⌜Φ v⌝ }})) →
+     ⊢ |={⊤}=> ∀ name_map_name,
+         ∃
+         (stateI : nat → state M → iProp Σ),
+         let _ : irisG M Σ := IrisG _ _ Hinv _ _ _ name_map_name stateI in
+         |={⊤}=> ∃ (Ps : list (iProp Σ)),
+       ⌜length Ps = length ms⌝ ∗
+       stateI (length ms) σ ∗
+       (([∗ list] id ↦ P ∈ Ps, VMProp id P) -∗
+           [∗ list] id ↦ m;Φ ∈ ms;φs,
+             if terminated m then
+                ⌜Φ m⌝
+              else (if (scheduled σ id) then True else VMProp_holds id) -∗
+              WP m @ id; ⊤ {{v, ⌜Φ v⌝ }})) →
   adequate ms σ ((λ φ, λ v _, φ v)<$> φs).
 Proof.
-  intros Hwp. apply adequate_alt. intros ms2 σ2 [n ?]%rtc_nsteps.
+  intros Hlen Hwp. apply adequate_alt. intros ms2 σ2 [n ?]%rtc_nsteps.
   eapply (wp_strong_adequacy Σ M); [|done]=> ?.
-  iMod Hwp as (stateI) "[Hσ Hwp]".
+  iMod Hwp as "Hwp"; clear Hwp.
+  iModIntro.
+  iIntros (name_map_name).
+  iDestruct ("Hwp" $! name_map_name) as (stateI) "Hwp".
   iExists stateI, ((λ φ, λ v, ⌜φ v⌝) <$> φs)%I.
-  rewrite !big_sepL2_fmap_r.
-  iIntros "{$Hσ $Hwp} !>" (?) "_ H".
-  iApply fupd_mask_intro_discard; [done|]. iSplit; [|done].
-  iDestruct (big_sepL2_length with "H") as %Hlength.
+  iMod "Hwp" as (Ps) "(%HPs & Hσ & Hwp)".
+  iModIntro. iExists _; iSplit; first done; iFrame "Hσ".
+  iSplitL.
+  { rewrite !big_sepL2_fmap_r.
+    iFrame. }
+  iIntros (Hnstk) "Hsi Hpost".
+  iApply fupd_mask_intro_discard; first set_solver.
+  iSplit; last done.
   rewrite Forall2_lookup.
   iIntros (i).
   rewrite list_lookup_fmap.
   destruct (ms2 !! i) eqn:Hi.
   - destruct (lookup_lt_is_Some_2 φs i) as [φ Hφ].
-    { rewrite -Hlength; eapply lookup_lt_Some; done. }
+    { rewrite -Hlen.
+      erewrite nsteps_preserve_vms_length; last done.
+      eapply lookup_lt_Some; done. }
     rewrite Hφ /=.
-    rewrite /= big_sepL2_lookup; [|done|done].
+    rewrite /= big_sepL2_lookup; [|done|rewrite list_lookup_fmap Hφ; done].
     destruct (terminated m) eqn:Hmterm.
-    + iDestruct "H" as %?.
+    + iDestruct "Hpost" as %?.
       iPureIntro. apply Some_Forall2.
       rewrite Hmterm; done.
     + iPureIntro. apply Some_Forall2.
       rewrite Hmterm; done.
   - rewrite (lookup_ge_None_2 φs i); last first.
-    { rewrite -Hlength; eapply lookup_ge_None_1; done. }
+    { rewrite -Hlen.
+      erewrite nsteps_preserve_vms_length; last done.
+      eapply lookup_ge_None_1; done. }
     iPureIntro. apply None_Forall2.
 Qed.
 
-Corollary wp_invariance Σ M `{!invGpreS Σ} ms1 σ1 ms2 σ2 φ :
+Corollary wp_invariance Σ M `{!irisPreGS Σ} ms1 σ1 ms2 σ2 φ :
   (∀ `{Hinv : !invGS Σ},
-     ⊢ |={⊤}=> ∃
-         (stateI : state M → iProp Σ),
-       let _ : irisG M Σ := IrisG _ _ Hinv stateI in
-       stateI σ1 ∗ ([∗ list] id ↦ e ∈ ms1, WP e @ id; ⊤ {{v, True }}) ∗
-       (stateI σ2 -∗ ∃ E, |={⊤,E}=> ⌜φ⌝)) →
+     ⊢ |={⊤}=> ∀ name_map_name,
+         ∃
+         (stateI : nat → state M → iProp Σ),
+         let _ : irisG M Σ := IrisG _ _ Hinv _ _ _ name_map_name stateI in
+         |={⊤}=> ∃ (Ps : list (iProp Σ)),
+       ⌜length Ps = length ms1⌝ ∗
+       stateI (length ms1) σ1 ∗
+       (([∗ list] id ↦ P ∈ Ps, VMProp id P) -∗
+           [∗ list] id ↦ m ∈ ms1,
+             if terminated m then
+                True
+              else (if (scheduled σ1 id) then True else VMProp_holds id) -∗
+              WP m @ id; ⊤ {{_, True }}) ∗
+       (stateI (length ms2) σ2 -∗ ∃ E, |={⊤,E}=> ⌜φ⌝)) →
   rtc step (ms1, σ1) (ms2, σ2) →
   φ.
 Proof.
   intros Hwp [n Hmss]%rtc_nsteps.
-  assert (length ms1 = length ms2).
+  assert (length ms1 = length ms2) as Hms1ms2len.
   { clear -Hmss.
     change ms1 with ((ms1, σ1).1).
     change ms2 with ((ms2, σ2).1).
     induction Hmss as [|? [] [] ??? <-]; first done.
     eapply step_length; done. }
   eapply (wp_strong_adequacy Σ _); [|done]=> ?.
-  iMod (Hwp _) as (stateI) "(Hσ & Hwp & Hφ)".
+  iMod Hwp as "Hwp".
+  iModIntro.
+  iIntros (name_map_name).
+  iDestruct ("Hwp" $! name_map_name) as (stateI) "Hwp".
   iExists stateI, (replicate (length ms1) (λ _, True))%I.
+  iMod "Hwp" as (Ps Hlen) "(Hσ & Hwp & Hφ)".
+  iModIntro.
+  iExists _; iSplit; first done.
+  iFrame "Hσ".
   rewrite !big_sepL2_replicate_r; [|done|done].
-  iIntros "{$Hσ $Hwp} !>" (?) "Hσ H /=".
+  iFrame "Hwp".
+  iIntros (?) "Hσ H /=".
+  rewrite Hms1ms2len.
   iDestruct ("Hφ" with "Hσ") as (E) ">Hφ".
   by iApply fupd_mask_intro_discard; first set_solver.
 Qed.
